cfrontend/BeePL_auxlemmas.v
@@ -2,36 +2,117 @@ Require Import String ZArith Coq.FSets.FMapAVL Coq.Structures.OrderedTypeEx FunI
 Require Import Coq.FSets.FSetProperties Coq.FSets.FMapFacts FMaps FSetAVL Nat PeanoNat Linking.
 Require Import Coq.Arith.EqNat Coq.ZArith.Int Integers AST Maps Linking Ctypes Smallstep SimplExpr.
 Require Import BeePL_aux BeePL_mem BeeTypes BeePL Csyntax Clight Globalenvs BeePL_Csyntax SimplExpr.
-Require Import compcert.common.Errors Initializersproof Cstrategy lib.Coqlib Errors.
-
-From mathcomp Require Import all_ssreflect. 
+Require Import Errors Initializersproof Cstrategy Coqlib Errors.
 
 Lemma access_mode_preserved : forall ty cty md, 
 access_mode ty = md ->
 transBeePL_type ty = OK cty ->
 Ctypes.access_mode cty = md.
 Proof.
-Admitted.
+  intros ty cty md HACCESS HTRANS.
+  destruct ty eqn:Ety; simpl in HACCESS.
+  (* Case: Ptype *)
+  - destruct p eqn:Ep; simpl in *.
+    (* Tunit *)
+    + monadInv HTRANS. reflexivity.
+    (* Tint *)
+    + destruct i; destruct s; monadInv HTRANS; eauto.
+    (* Tlong *)
+    + destruct s; monadInv HTRANS; eauto.
+  (* Case: Reftype *)
+  - destruct b; simpl in *;
+    destruct p; simpl in *;
+    monadInv HTRANS;
+    eauto.
+  (* Case: Ftype *)
+  - monadInv HTRANS.
+    destruct (transBeePL_types transBeePL_type l) eqn:?;
+    try discriminate.
+    destruct (transBeePL_type t) eqn:?; try discriminate.
+    reflexivity.
+Qed.
+
 
 Lemma non_volatile_type_preserved : forall ty cty,
 type_is_volatile ty = false ->
 transBeePL_type ty = OK cty ->
 Ctypes.type_is_volatile cty = false.
 Proof.
-Admitted.
+  intros ty cty HNVOL HTRANS.
+  destruct ty eqn:Ety; simpl in *.
+  (* Case: Ptype *)
+  - destruct p; simpl in *; monadInv HTRANS; eauto.
+  (* Case: Reftype *)
+  - destruct b; destruct p; simpl in *;
+    monadInv HTRANS; eauto.
+  (* Case: Ftype *)
+  - monadInv HTRANS.
+    destruct (transBeePL_types transBeePL_type l) eqn:?;
+    try discriminate.
+    destruct (transBeePL_type t) eqn:?; try discriminate.
+    eauto.
+Qed.
+
 
 Lemma typec_expr : forall e ct ce,
 transBeePL_type (typeof_expr e) = OK ct ->
 transBeePL_expr_expr e = OK ce ->
 ct = Csyntax.typeof ce.
 Proof.
-Admitted.
+  induction e; simpl; intros.
+  (* Case: Val *)
+  - monadInv H0.
+    rewrite EQ in H. inv H.
+    reflexivity.
+  (* Case: Valof *)
+  - monadInv H0.
+    rewrite EQ in H. inv H.
+    reflexivity.
+  (* Case: Var *)
+  - monadInv H0.
+    rewrite EQ in H. inv H.
+    reflexivity.
+  (* Case: Const *)
+  - destruct c; monadInv H0;
+    rewrite EQ in H; inv H;
+    reflexivity.
+  (* Case: App *)
+  - monadInv H0.
+    rewrite EQ0 in H. inv H.
+    reflexivity.
+  (* Case: Prim *)
+  - destruct b eqn:Eb; monadInv H0; try discriminate;
+    try (rewrite EQ1 in H; inv H; reflexivity).
+    (* Want to double check the case for Run*)
+    rewrite EQ in H. inv H. reflexivity.
+  (* Case: Bind *)
+  - monadInv H0.
+    rewrite EQ2 in H. inv H.
+    reflexivity.
+  (* Case: Cond *)
+  - monadInv H0.
+    rewrite EQ2 in H. inv H.
+    reflexivity.
+  (* Case: Unit *)
+  - monadInv H0.
+    rewrite EQ in H. inv H.
+    reflexivity.
+  (* Case: Addr *)
+  - monadInv H0.
+    rewrite EQ in H. inv H.
+    reflexivity.
+  (* Case: Hexpr FIX ME *)
+  - monadInv H0.
+    rewrite EQ in H. inv H.
+    reflexivity.
+Qed.
+
 
 Lemma bv_cv_reflex : forall v' v,
 transC_val_bplvalue v' = OK v ->
 transBeePL_value_cvalue v = v'.
 Proof.
-Admitted.
-
-
-
+  intros v' v H.
+  destruct v' eqn:?; simpl in *; try discriminate;
+  inv H; reflexivity.
+Qed.
